src/theory/bin_hoare_logic/bin_hoare_logicScript.sml
@@ -41,7 +41,7 @@ val weak_comp_thm = prove(``
   !m.
   weak_model m ==>
   !ms ls1 ls2 ms' ms''.
-  (m.weak ms (ls1 UNION ls2) ms') ==> (~ ((m.pc ms') IN ls2)) ==>
+  (m.weak ms (ls1 UNION ls2) ms') ==> (~((m.pc ms') IN ls2)) ==>
   (m.weak ms' ls2 ms'') ==> (m.weak ms ls2 ms'')``,
 
 REPEAT STRIP_TAC >>
